Weidenbach_Book/IsaSAT/IsaSAT_VDom_LLVM.thy
@@ -6,7 +6,7 @@ no_notation WB_More_Refinement.freft (\<open>_ \<rightarrow>\<^sub>f _\<close> [
 
 type_synonym aivdom2 = \<open>vdom \<times> vdom \<times> vdom\<close>
 abbreviation aivdom_int_rel :: \<open>(aivdom2 \<times> aivdom) set\<close> where
-  \<open>aivdom_int_rel \<equiv> {(a, (_, a')). (a,a') \<in> \<langle>Id\<rangle>list_rel \<times>\<^sub>r \<langle>Id\<rangle>list_rel \<times>\<^sub>r \<langle>Id\<rangle>list_rel}\<close>
+  \<open>aivdom_int_rel \<equiv> {(a, (_, a')). (a,a') \<in> \<langle>nat_rel\<rangle>list_rel \<times>\<^sub>r \<langle>nat_rel\<rangle>list_rel \<times>\<^sub>r \<langle>nat_rel\<rangle>list_rel}\<close>
 
 abbreviation aivdom_rel :: \<open>(aivdom2 \<times> isasat_aivdom) set\<close> where
   \<open>aivdom_rel \<equiv> \<langle>aivdom_int_rel\<rangle>code_hider_rel\<close>
@@ -17,6 +17,7 @@ type_synonym aivdom_assn = \<open>vdom_fast_assn \<times> vdom_fast_assn \<times
 definition aivdom_assn :: \<open>isasat_aivdom \<Rightarrow> _ \<Rightarrow> assn\<close> where
   \<open>aivdom_assn = code_hider_assn aivdom_int_assn aivdom_int_rel\<close>
 
+text \<open>To keep my sanity, I use the same name, even if the function drops one component.\<close>
 definition add_learned_clause_aivdom_int where
   \<open>add_learned_clause_aivdom_int = (\<lambda> C (avdom, ivdom). (avdom @ [C], ivdom))\<close>
 
@@ -41,6 +42,27 @@ definition length_tvdom_aivdom_int :: \<open>aivdom2 \<Rightarrow> nat\<close> w
 
 definition length_avdom_aivdom_int :: \<open>aivdom2 \<Rightarrow> nat\<close> where
   \<open>length_avdom_aivdom_int = (\<lambda>(b,c,d). length b)\<close>
+
+definition AIVDom_int :: \<open>_ \<Rightarrow> _ \<Rightarrow> _ \<Rightarrow> _ \<Rightarrow> aivdom2\<close> where
+  \<open>AIVDom_int _ avdom ivdom tvdom = (avdom, ivdom, tvdom)\<close>
+
+definition swap_avdom_aivdom_int :: \<open>aivdom2 \<Rightarrow> nat \<Rightarrow> nat \<Rightarrow> aivdom2\<close> where
+  \<open>swap_avdom_aivdom_int = (\<lambda>(avdom, ivdom, tvdom) i j.
+  (swap avdom i j, ivdom, tvdom))\<close>
+
+lemma swap_avdom_aivdom_alt_def:
+  \<open>swap_avdom_aivdom aivdom i j =
+  (AIvdom (get_vdom_aivdom aivdom, swap (get_avdom_aivdom aivdom) i j, get_ivdom_aivdom aivdom, get_tvdom_aivdom aivdom))\<close>
+  by (cases aivdom) auto
+
+definition take_avdom_aivdom_int :: \<open>nat \<Rightarrow> aivdom2 \<Rightarrow> aivdom2\<close> where
+  \<open>take_avdom_aivdom_int = (\<lambda>i (avdom, ivdom, tvdom).
+  (take i avdom, ivdom, tvdom))\<close>
+
+lemma take_avdom_aivdom_alt_def:
+  \<open>take_avdom_aivdom i aivdom =
+  (AIvdom (get_vdom_aivdom aivdom, take i (get_avdom_aivdom aivdom), get_ivdom_aivdom aivdom, get_tvdom_aivdom aivdom))\<close>
+  by (cases aivdom) auto
   
 lemma
   add_learned_clause_aivdom_int:
@@ -58,8 +80,14 @@ lemma
   length_ivdom_aivdom_int:
   \<open>(RETURN o length_ivdom_aivdom_int, RETURN o length_ivdom_aivdom) \<in> aivdom_rel \<rightarrow>\<^sub>f \<langle>nat_rel\<rangle>nres_rel\<close> and
   length_tvdom_aivdom_int:
-  \<open>(RETURN o length_tvdom_aivdom_int, RETURN o length_tvdom_aivdom) \<in> aivdom_rel \<rightarrow>\<^sub>f \<langle>nat_rel\<rangle>nres_rel\<close>
-  by (auto intro!: frefI nres_relI simp: code_hider_rel_def add_learned_clause_aivdom_def remove_inactive_aivdom_def avdom_aivdom_at_alt_def
+  \<open>(RETURN o length_tvdom_aivdom_int, RETURN o length_tvdom_aivdom) \<in> aivdom_rel \<rightarrow>\<^sub>f \<langle>nat_rel\<rangle>nres_rel\<close> and
+  swap_avdom_aivdom_int:
+  \<open>(uncurry2 (RETURN ooo swap_avdom_aivdom_int), uncurry2 (RETURN ooo swap_avdom_aivdom))
+  \<in> aivdom_rel \<times>\<^sub>f nat_rel \<times>\<^sub>f nat_rel  \<rightarrow>\<^sub>f \<langle>aivdom_rel\<rangle>nres_rel\<close> and
+  take_avdom_aivdom_int:
+  \<open>(uncurry (RETURN oo take_avdom_aivdom_int), uncurry (RETURN oo take_avdom_aivdom))
+  \<in> nat_rel \<times>\<^sub>f aivdom_rel  \<rightarrow>\<^sub>f \<langle>aivdom_rel\<rangle>nres_rel\<close>
+  apply (auto intro!: frefI nres_relI simp: code_hider_rel_def add_learned_clause_aivdom_def remove_inactive_aivdom_def avdom_aivdom_at_alt_def
     ivdom_aivdom_at_alt_def vdom_aivdom_at_alt_def length_vdom_aivdom_alt_def length_avdom_aivdom_alt_def length_ivdom_aivdom_alt_def length_tvdom_aivdom_alt_def tvdom_aivdom_at_alt_def add_learned_clause_aivdom_int_def
     IsaSAT_VDom.add_learned_clause_aivdom_int_def
     IsaSAT_VDom.remove_inactive_aivdom_int_def remove_inactive_aivdom_int_def
@@ -69,11 +97,14 @@ lemma
     IsaSAT_VDom.length_avdom_aivdom_int_def length_avdom_aivdom_int_def
     IsaSAT_VDom.length_ivdom_aivdom_int_def length_ivdom_aivdom_int_def
     IsaSAT_VDom.length_tvdom_aivdom_int_def length_tvdom_aivdom_int_def
-    )
+    swap_avdom_aivdom_alt_def)
+   apply (case_tac ab; auto simp: swap_avdom_aivdom_int_def take_avdom_aivdom_int_def)
+   apply (case_tac ba; auto simp: swap_avdom_aivdom_int_def take_avdom_aivdom_int_def)
+   done
 
 sepref_def add_learned_clause_aivdom_impl
   is \<open>uncurry (RETURN oo add_learned_clause_aivdom_int)\<close>
-  :: \<open>[\<lambda>(C,(a,b,c)). Suc (length (a)) < max_snat 64 \<and> Suc (length b) < max_snat 64]\<^sub>a sint64_nat_assn\<^sup>k *\<^sub>a aivdom_int_assn\<^sup>d \<rightarrow> aivdom_int_assn\<close>
+  :: \<open>[\<lambda>(C,(a,b,c)). Suc (length (a)) < max_snat 64]\<^sub>a sint64_nat_assn\<^sup>k *\<^sub>a aivdom_int_assn\<^sup>d \<rightarrow> aivdom_int_assn\<close>
   unfolding add_learned_clause_aivdom_int_def
   by sepref
 
@@ -124,21 +155,26 @@ sepref_def length_ivdom_aivdom_impl
   unfolding length_ivdom_aivdom_int_def comp_def workaround_RF_def[symmetric]
   by sepref
 
-sepref_def length_vdom_aivdom_impl
-  is \<open>RETURN o length_vdom_aivdom_int\<close>
-  :: \<open>aivdom_int_assn\<^sup>k \<rightarrow>\<^sub>a sint64_nat_assn\<close>
-  unfolding length_vdom_aivdom_int_def
-  by sepref
-
 sepref_def length_tvdom_aivdom_impl
   is \<open>RETURN o length_tvdom_aivdom_int\<close>
   :: \<open>aivdom_int_assn\<^sup>k \<rightarrow>\<^sub>a sint64_nat_assn\<close>
   unfolding length_tvdom_aivdom_int_def comp_def workaround_RF_def[symmetric]
   by sepref
 
+sepref_def swap_avdom_aivdom_impl
+  is \<open>uncurry2 (RETURN ooo swap_avdom_aivdom_int)\<close>
+  :: \<open>[\<lambda>(((b,c,d),i), j). i < length b \<and> j < length b]\<^sub>a aivdom_int_assn\<^sup>d *\<^sub>a sint64_nat_assn\<^sup>k *\<^sub>a sint64_nat_assn\<^sup>k \<rightarrow> aivdom_int_assn\<close>
+  unfolding swap_avdom_aivdom_int_def convert_swap gen_swap
+  by sepref
+
+sepref_def take_avdom_aivdom_impl
+  is \<open>uncurry (RETURN oo take_avdom_aivdom_int)\<close>
+  :: \<open>[\<lambda>(i, (b,c,d)). i \<le> length b]\<^sub>a sint64_nat_assn\<^sup>k *\<^sub>a aivdom_int_assn\<^sup>d \<rightarrow> aivdom_int_assn\<close>
+  unfolding take_avdom_aivdom_int_def
+  by sepref
+
 lemma aivdom_assn_alt_def:
-  \<open>aivdom_assn = hr_comp aivdom_int_assn
-  (\<langle>\<langle>nat_rel\<rangle>list_rel \<times>\<^sub>r \<langle>nat_rel\<rangle>list_rel \<times>\<^sub>r \<langle>nat_rel\<rangle>list_rel \<times>\<^sub>r \<langle>nat_rel\<rangle>list_rel\<rangle>code_hider_rel)\<close>
+  \<open>aivdom_assn = hr_comp aivdom_int_assn (\<langle>aivdom_int_rel\<rangle>code_hider_rel)\<close>
   unfolding aivdom_assn_def code_hider_assn_def by auto
 
 context
@@ -147,20 +183,16 @@ begin
 
 theorem [sepref_fr_rules]:
   \<open>(uncurry add_learned_clause_aivdom_impl, uncurry (RETURN \<circ>\<circ> add_learned_clause_aivdom))
-\<in> [\<lambda>(C,ai). Suc (length (get_vdom_aivdom ai)) < max_snat 64 \<and> Suc (length (get_avdom_aivdom ai)) < max_snat 64]\<^sub>a snat_assn\<^sup>k *\<^sub>a aivdom_assn\<^sup>d \<rightarrow> aivdom_assn\<close>
+\<in> [\<lambda>(C,ai). Suc (length (get_avdom_aivdom ai)) < max_snat 64]\<^sub>a snat_assn\<^sup>k *\<^sub>a aivdom_assn\<^sup>d \<rightarrow> aivdom_assn\<close>
   (is \<open>?c \<in> [?pre]\<^sub>a ?im \<rightarrow> ?f\<close>)
 proof -
   have H: \<open>?c
-\<in> [comp_PRE
-    (nat_rel \<times>\<^sub>f \<langle>\<langle>nat_rel\<rangle>list_rel \<times>\<^sub>r \<langle>nat_rel\<rangle>list_rel \<times>\<^sub>f (\<langle>nat_rel\<rangle>list_rel \<times>\<^sub>f \<langle>nat_rel\<rangle>list_rel)\<rangle>code_hider_rel)
-    (\<lambda>_. True)
-    (\<lambda>x y. case y of (C, a, b, c) \<Rightarrow> Suc (length a) < max_snat 64 \<and> Suc (length b) < max_snat 64)
-    (\<lambda>x. nofail
-    (uncurry (RETURN \<circ>\<circ> add_learned_clause_aivdom)
-      x))]\<^sub>a ?im \<rightarrow> ?f\<close>
+\<in> [comp_PRE (nat_rel \<times>\<^sub>f aivdom_rel) (\<lambda>_. True)
+   (\<lambda>x y. case y of (C, a, b, c) \<Rightarrow> Suc (length a) < max_snat 64)
+   (\<lambda>x. nofail (uncurry (RETURN \<circ>\<circ> add_learned_clause_aivdom) x))]\<^sub>a ?im \<rightarrow> ?f\<close>
     (is \<open>_ \<in> [?pre']\<^sub>a _ \<rightarrow> _\<close>)
     using hfref_compI_PRE[OF add_learned_clause_aivdom_impl.refine
-      add_learned_clause_aivdom_int, unfolded fcomp_norm_unfold aivdom_assn_alt_def[symmetric]] by simp
+      add_learned_clause_aivdom_int, unfolded fcomp_norm_unfold aivdom_assn_alt_def[symmetric]] by blast
   have pre: \<open>?pre' = ?pre\<close> for x h
     by (intro ext, rename_tac x, case_tac x, case_tac \<open>snd x\<close>)
       (auto simp: comp_PRE_def code_hider_rel_def)
@@ -178,14 +210,12 @@ theorem [sepref_fr_rules]:
 proof -
   have H: \<open>?c
 \<in> [comp_PRE
-   (nat_rel \<times>\<^sub>f \<langle>\<langle>nat_rel\<rangle>list_rel \<times>\<^sub>r \<langle>nat_rel\<rangle>list_rel \<times>\<^sub>f (\<langle>nat_rel\<rangle>list_rel \<times>\<^sub>f \<langle>nat_rel\<rangle>list_rel)\<rangle>code_hider_rel)
-   (\<lambda>_. True) (\<lambda>x y. case y of (C, a, b, c) \<Rightarrow> C < length b)
-   (\<lambda>x. nofail
-      (uncurry (RETURN \<circ>\<circ> remove_inactive_aivdom)
-        x))]\<^sub>a ?im \<rightarrow> ?f\<close>
+   (nat_rel \<times>\<^sub>f aivdom_rel)
+   (\<lambda>_. True) (\<lambda>x y. case y of (C, a, b, c) \<Rightarrow> C < length a)
+   (\<lambda>x. nofail (uncurry (RETURN \<circ>\<circ> remove_inactive_aivdom) x))]\<^sub>a ?im \<rightarrow> ?f\<close>
     (is \<open>_ \<in> [?pre']\<^sub>a _ \<rightarrow> _\<close>)
     using hfref_compI_PRE[OF remove_inactive_aivdom_impl.refine
-      remove_inactive_aivdom_int, unfolded fcomp_norm_unfold aivdom_assn_alt_def[symmetric]] by simp
+      remove_inactive_aivdom_int, unfolded fcomp_norm_unfold aivdom_assn_alt_def[symmetric]] by blast
   have pre: \<open>?pre' = ?pre\<close> for x h
     by (intro ext, rename_tac x, case_tac x, case_tac \<open>snd x\<close>)
       (auto simp: comp_PRE_def code_hider_rel_def)
@@ -203,8 +233,8 @@ theorem [sepref_fr_rules]:
 proof -
   have H: \<open>?c
 \<in> [comp_PRE
-    (\<langle>\<langle>nat_rel\<rangle>list_rel \<times>\<^sub>f (\<langle>nat_rel\<rangle>list_rel \<times>\<^sub>r \<langle>nat_rel\<rangle>list_rel \<times>\<^sub>f \<langle>nat_rel\<rangle>list_rel)\<rangle>code_hider_rel \<times>\<^sub>f nat_rel)
-    (\<lambda>_. True) (\<lambda>x y. case y of (x, xa) \<Rightarrow> (case x of (a, b, c) \<Rightarrow> \<lambda>C. C < length b) xa)
+    (aivdom_rel \<times>\<^sub>f nat_rel)
+    (\<lambda>_. True) (\<lambda>x y. case y of (x, xa) \<Rightarrow> (case x of (b, c) \<Rightarrow> \<lambda>C. C < length b) xa)
     (\<lambda>x. nofail
     (uncurry (RETURN \<circ>\<circ> avdom_aivdom_at) x))]\<^sub>a ?im \<rightarrow> ?f\<close>
     (is \<open>_ \<in> [?pre']\<^sub>a _ \<rightarrow> _\<close>)
@@ -227,8 +257,8 @@ theorem [sepref_fr_rules]:
 proof -
   have H: \<open>?c
 \<in> [comp_PRE
-    (\<langle>\<langle>nat_rel\<rangle>list_rel \<times>\<^sub>f (\<langle>nat_rel\<rangle>list_rel \<times>\<^sub>r \<langle>nat_rel\<rangle>list_rel \<times>\<^sub>f \<langle>nat_rel\<rangle>list_rel)\<rangle>code_hider_rel \<times>\<^sub>f nat_rel)
-    (\<lambda>_. True) (\<lambda>x y. case y of (x, xa) \<Rightarrow> (case x of (a, b, c, d) \<Rightarrow> \<lambda>C. C < length c) xa)
+    (\<langle>aivdom_int_rel\<rangle>code_hider_rel \<times>\<^sub>f nat_rel)
+    (\<lambda>_. True) (\<lambda>x y. case y of (x, xa) \<Rightarrow> (case x of (b, c, d) \<Rightarrow> \<lambda>C. C < length c) xa)
     (\<lambda>x. nofail
     (uncurry (RETURN \<circ>\<circ> ivdom_aivdom_at) x))]\<^sub>a ?im \<rightarrow> ?f\<close>
     (is \<open>_ \<in> [?pre']\<^sub>a _ \<rightarrow> _\<close>)
@@ -251,15 +281,13 @@ theorem [sepref_fr_rules]:
 proof -
   have H: \<open>?c
 \<in> [comp_PRE
-   (\<langle>\<langle>nat_rel\<rangle>list_rel \<times>\<^sub>f
-     (\<langle>nat_rel\<rangle>list_rel \<times>\<^sub>f (\<langle>nat_rel\<rangle>list_rel \<times>\<^sub>f \<langle>nat_rel\<rangle>list_rel))\<rangle>code_hider_rel \<times>\<^sub>f
-    nat_rel)
-   (\<lambda>_. True) (\<lambda>x y. case y of (x, xa) \<Rightarrow> (case x of (a, b, c, d) \<Rightarrow> \<lambda>C. C < length d) xa)
+   (aivdom_rel \<times>\<^sub>f nat_rel)
+   (\<lambda>_. True) (\<lambda>x y. case y of (x, xa) \<Rightarrow> (case x of (b, c, d) \<Rightarrow> \<lambda>C. C < length d) xa)
    (\<lambda>x. nofail
       (uncurry (RETURN \<circ>\<circ> tvdom_aivdom_at) x))]\<^sub>a ?im \<rightarrow> ?f\<close>
     (is \<open>_ \<in> [?pre']\<^sub>a _ \<rightarrow> _\<close>)
     using hfref_compI_PRE[OF tvdom_aivdom_at_impl.refine
-      tvdom_aivdom_at_int, unfolded fcomp_norm_unfold aivdom_assn_alt_def[symmetric]] by simp
+      tvdom_aivdom_at_int, unfolded fcomp_norm_unfold aivdom_assn_alt_def[symmetric]] by blast
   have pre: \<open>?pre' = ?pre\<close> for x h
     by (intro ext, rename_tac x, case_tac x, case_tac \<open>fst x\<close>)
       (auto simp: comp_PRE_def code_hider_rel_def)
@@ -270,14 +298,67 @@ proof -
 qed
 
 
+theorem [sepref_fr_rules]:
+  \<open>(uncurry take_avdom_aivdom_impl, uncurry (RETURN \<circ>\<circ> take_avdom_aivdom))
+\<in> [\<lambda>(C, ai). C \<le> length (get_avdom_aivdom ai)]\<^sub>a sint64_nat_assn\<^sup>k *\<^sub>a aivdom_assn\<^sup>d \<rightarrow> aivdom_assn\<close>
+  (is \<open>?c \<in> [?pre]\<^sub>a ?im \<rightarrow> ?f\<close>)
+proof -
+  have H: \<open>?c
+\<in> [comp_PRE (nat_rel \<times>\<^sub>f aivdom_rel) (\<lambda>_. True)
+    (\<lambda>x y. case y of (i, b, c, d) \<Rightarrow> i \<le> length b)
+    (\<lambda>x. nofail (uncurry (RETURN \<circ>\<circ> take_avdom_aivdom) x))]\<^sub>a ?im \<rightarrow> ?f\<close>
+    (is \<open>_ \<in> [?pre']\<^sub>a _ \<rightarrow> _\<close>)
+    using hfref_compI_PRE[OF take_avdom_aivdom_impl.refine
+      take_avdom_aivdom_int, unfolded fcomp_norm_unfold aivdom_assn_alt_def[symmetric]] by blast
+  have pre: \<open>?pre' = ?pre\<close> for x h
+    by (intro ext, rename_tac x, case_tac x, case_tac \<open>snd x\<close>)
+      (auto simp: comp_PRE_def code_hider_rel_def)
+  show ?thesis
+    using H
+    unfolding pre
+    by blast
+qed
+
+
+theorem [sepref_fr_rules]:
+  \<open>(uncurry2 swap_avdom_aivdom_impl, uncurry2 (RETURN ooo swap_avdom_aivdom))
+  \<in> [\<lambda>((ai, i), j). i < length (get_avdom_aivdom ai) \<and> j < length (get_avdom_aivdom ai)]\<^sub>a
+  aivdom_assn\<^sup>d   *\<^sub>a sint64_nat_assn\<^sup>k *\<^sub>a sint64_nat_assn\<^sup>k \<rightarrow> aivdom_assn\<close>
+  (is \<open>?c \<in> [?pre]\<^sub>a ?im \<rightarrow> ?f\<close>)
+proof -
+  have H: \<open>?c
+\<in> [comp_PRE (aivdom_rel \<times>\<^sub>f nat_rel \<times>\<^sub>f nat_rel) (\<lambda>_. True)
+    (\<lambda>x y. case y of
+     (x, xa) \<Rightarrow>
+       (case x of
+        (x, xa) \<Rightarrow>
+       (case x of
+        (b, c, d) \<Rightarrow> \<lambda>i j. i < length b \<and> j < length b)
+        xa)
+        xa)
+    (\<lambda>x. nofail
+    (uncurry2 (RETURN \<circ>\<circ>\<circ> swap_avdom_aivdom)
+      x))]\<^sub>a ?im \<rightarrow> ?f\<close>
+    (is \<open>_ \<in> [?pre']\<^sub>a _ \<rightarrow> _\<close>)
+    using hfref_compI_PRE[OF swap_avdom_aivdom_impl.refine
+      swap_avdom_aivdom_int, unfolded fcomp_norm_unfold aivdom_assn_alt_def[symmetric]] by blast
+  have pre: \<open>?pre' = ?pre\<close> for x h
+    by (intro ext, rename_tac x, case_tac x, case_tac \<open>fst (fst x)\<close>)
+      (auto simp: comp_PRE_def code_hider_rel_def)
+  show ?thesis
+    using H
+    unfolding pre
+    by blast
+qed
+
 lemma aivdom_int_assn_alt_def:
   \<open>aivdom_int_assn = hr_comp aivdom_int_assn
-  (\<langle>nat_rel\<rangle>list_rel \<times>\<^sub>r \<langle>nat_rel\<rangle>list_rel \<times>\<^sub>f (\<langle>nat_rel\<rangle>list_rel \<times>\<^sub>f \<langle>nat_rel\<rangle>list_rel))\<close>
+  (\<langle>nat_rel\<rangle>list_rel \<times>\<^sub>f (\<langle>nat_rel\<rangle>list_rel \<times>\<^sub>f \<langle>nat_rel\<rangle>list_rel))\<close>
   by auto
 
+sepref_register swap_avdom_aivdom take_avdom_aivdom
 lemmas [sepref_fr_rules] =
   length_avdom_aivdom_impl.refine[FCOMP length_avdom_aivdom_int]
-  length_vdom_aivdom_impl.refine[FCOMP length_vdom_aivdom_int]
   length_ivdom_aivdom_impl.refine[FCOMP length_ivdom_aivdom_int]
   length_tvdom_aivdom_impl.refine[FCOMP length_tvdom_aivdom_int]
   hn_id[FCOMP Constructor_hnr[of aivdom_int_rel], of aivdom_int_assn,
